---
title: "zTest"
---

$$
\begin{align}
\E(\hat\beta | X, z) & = \beta + (X^\top X)^{-1}X^\top z \delta\\
& = \beta + \color{blue}{\hat\eta}\color{black}\delta && (\because \color{blue}{\hat\eta = (X^\top X)^{-1} X^\top z }\color{black}) \\
\E\hat\beta & = \E(\E(\hat\beta|X, z)) && \text{(law of iterated expect.)} \\
& = E(\color{blue}{\beta + \hat\eta \delta}\color{black}) && (\because \color{blue}{\E(\hat\beta|X, z) = \beta + \hat\eta\delta} \color{black}) \\
& = \beta + \E\hat\eta \ \delta && \text{(take out constants from exp.)} \\
& = \beta + \eta\delta && (\text{unbiased estimator } \E\hat\eta = \eta)
\end{align}
$$

$$
\hat\beta_1 = (\tilde X_1^\top \tilde X_1)^{-1}\tilde X_1 ^\top \tilde y
$$